fstar/MLS.TreeSync.KeyPackageRef.fst
@@ -13,23 +13,3 @@ val compute_key_package_ref: #bytes:Type0 -> {|crypto_bytes bytes|} -> key_packa
 let compute_key_package_ref #bytes #cb kp =
   let kp_bytes: bytes = serialize (key_package_nt bytes) kp in
   make_keypackage_ref kp_bytes
-
-val compute_leaf_node_ref: #bytes:Type0 -> {|crypto_bytes bytes|} -> leaf_package_t bytes -> result (leaf_node_ref_nt bytes)
-let compute_leaf_node_ref #bytes #cb lp =
-  leaf <-- leaf_package_to_network lp;
-  let leaf_bytes: bytes = serialize (leaf_node_nt bytes) leaf in
-  make_leafnode_ref leaf_bytes
-
-val leaf_node_ref_to_index: #bytes:Type0 -> {|crypto_bytes bytes|} -> #l:nat -> #n:tree_size l -> treesync bytes l n -> leaf_node_ref_nt bytes -> result (option (leaf_index n))
-let leaf_node_ref_to_index #bytes #cb #l #n t ln_ref =
-  let leaves = get_leaf_list t in
-  ln_refs <-- mapM (fun olp ->
-    match olp with
-    | Some lp -> (
-        kp_ref <-- compute_leaf_node_ref #bytes #cb lp;
-        return (Some kp_ref)
-    )
-    | None -> return None
-  ) leaves;
-  let opt_res = (find_first (fun x -> x = Some ln_ref) ln_refs) in
-  return #(option (leaf_index n)) opt_res
